coq/theories/ITree/Delay.v
@@ -5,12 +5,12 @@ From OGS Require Import Utils.
 From OGS.Game Require Import Event.
 From OGS.ITree Require Import ITree.
 
-Definition delay (X : Type) : Type := itree ∅ₑ (X @ T1_0) T1_0.
+Definition delay (X : Type) : Type := itree ∅ₑ (fun _ => X) T1_0.
 
 Definition emb_delay {I} {E : event I I} {X i} : delay X -> itree E (X @ i) i :=
   cofix _emb_delay x :=
       go (match x.(_observe) with
-         | RetF (Fib r) => RetF (Fib r)
+         | RetF r => RetF (Fib r)
          | TauF t => TauF (_emb_delay t)
          | VisF e k => match e with end
          end).
